

5.

$$(a) \underline{b} \times \underline{\nabla} \times \underline{b} =$$

ASSUMING THIS MEANS:

$$= \underline{b} \times (\underline{\nabla} \times \underline{b}) = \epsilon_{ijk} b_j (\underline{\nabla} \times \underline{b})_k$$

$$= \epsilon_{ijk} b_j \epsilon_{klm} \partial_l b_m$$

$$= \epsilon_{kij} \epsilon_{klm} b_j \partial_l b_m$$

$$= (\delta_{il} \delta_{jm} - \delta_{im} \delta_{jl}) b_j \partial_l b_m$$

$$= b_m \partial_i b_m - b_l \partial_l b_i$$

~~$$= \partial_i (b_m b_m) - b_m \partial_i b_m - b_l \partial_l b_i$$~~

~~WHERE I HAVE USED~~

NOTE THAT:

$$\partial_i (b_m b_m) = b_m \partial_i b_m + b_m \partial_i b_m$$

$$= 2 b_m \partial_i b_m$$

$$\Rightarrow \partial_i \left(\frac{1}{2} b_m b_m \right) = b_m \partial_i b_m$$

USE THIS RESULT, REPLACE FIRST TERM:

$$= \partial_i \left(\frac{1}{2} b_m b_m \right) - b_l \partial_l b_i$$

$$= \underline{\nabla} \left(\frac{1}{2} \underline{b} \cdot \underline{b} \right) - \underline{b} \cdot \underline{\nabla} \underline{b}$$

NOW LET'S ASSUME ANOTHER ORDER =

$$\underline{b} \times \underline{\nabla} \times \underline{b} =$$

$$= (\underline{b} \times \underline{\nabla}) \times \underline{b} = \text{ ~~$\epsilon_{ijk} b_j \partial_k$~~ }$$

$$= \epsilon_{ijk} (\underline{b} \times \underline{\nabla})_j b_k$$

$$= \epsilon_{ijk} \epsilon_{jlm} b_l \partial_m b_k$$

$$\text{ ~~ϵ_{ijk}~~ }$$

$$= \epsilon_{jki} \epsilon_{jlm} b_l \partial_m b_k$$

$$\text{RELABEL: } j \rightarrow k, k \rightarrow i, i \rightarrow j.$$

$$= (\delta_{kl} \delta_{im} - \delta_{il} \delta_{km}) b_l \partial_m b_k$$

$$= b_k \partial_i b_k - b_i \partial_k b_k$$

$$= \underline{\nabla} \cdot \left(\frac{1}{2} \underline{b} \cdot \underline{b} \right) - \text{ ~~$\underline{b} \cdot \underline{\nabla} \cdot \underline{b}$~~ }$$

AS FOUND PREVIOUSLY,
SO WE'RE GOOD.

(b) $\nabla \times (\nabla a) =$

$$= \epsilon_{ijk} \partial_j (\nabla a)_k$$

$$= \epsilon_{ijk} \partial_j \partial_k a$$

THIS PART IS SYMMETRIC
UNDER $j \leftrightarrow k$ SWAP

THIS PART IS ANTISYMMETRIC
UNDER $j \leftrightarrow k$ SWAP

$$\Rightarrow \underline{\nabla \times (\nabla a) = 0}$$

(c) $\nabla \times (a \underline{b}) =$

$$= \epsilon_{ijk} \partial_j (a \underline{b})_k = \cancel{a \epsilon_{ijk} \partial_j b_k}$$

$$= \epsilon_{ijk} \partial_j (a b_k)$$

$$= \epsilon_{ijk} (a \partial_j b_k + b_k \partial_j a)$$

$$= a \epsilon_{ijk} \partial_j b_k + \cancel{b_k \epsilon_{ijk} \partial_j a} = \epsilon_{ikj} b_k \partial_j a$$

$$= a \nabla \times \underline{b} - \underline{b} \times \nabla a$$

"USING THE ABOVE IDENTITIES" ... PART

EULERIAN MOMENTUM EQUATION:

$$\rho \frac{\partial \underline{u}}{\partial t} + \rho (\underline{u} \cdot \nabla) \underline{u} = -\nabla p - \rho \nabla \Phi$$

CURL OF THIS:

$$\begin{aligned} \nabla \times \rho \frac{\partial \underline{u}}{\partial t} + \nabla \times \rho (\underline{u} \cdot \nabla) \underline{u} &= \\ &= \nabla \times (-\nabla p) - \nabla \times \rho \nabla \Phi \end{aligned}$$

RHS = 0 USING RESULT FROM b.

WE HAVE:

$$\nabla \times \rho \frac{\partial \underline{u}}{\partial t} + \nabla \times \rho (\underline{u} \cdot \nabla) \underline{u} = 0$$

$$\nabla \times \frac{\partial \underline{u}}{\partial t} + \nabla \times (\underline{u} \cdot \nabla) \underline{u} = 0$$

$$\frac{\partial}{\partial t} (\nabla \times \underline{u}) + \nabla \times (\underline{u} \cdot \nabla) \underline{u} = 0$$

~~BECAUSE THE PROBLEM SAYS~~

$$\nabla \times (\underline{u} \cdot \nabla) \underline{u} = 0$$

USING RESULTS FROM (a), REWRITE $(\underline{u} \cdot \nabla) \underline{u}$ AS:

$$\underline{u} \cdot \nabla \underline{u} = \nabla \left(\frac{1}{2} \underline{u} \cdot \underline{u} \right) - \underline{u} \times \nabla \times \underline{u}$$

REWRITE $\nabla \times (\underline{u} \cdot \nabla \underline{u})$ AS:

$$\nabla \times (\underline{u} \cdot \nabla \underline{u}) = \underbrace{\nabla \times \nabla \left(\frac{1}{2} \underline{u} \cdot \underline{u} \right)}_{=0 \text{ BY RESULT (b)}} - \nabla \times (\underline{u} \times \nabla \times \underline{u})$$

$$= \nabla \times (\underline{u} \times \nabla \times \underline{u})$$

WE HAVE

$$\frac{\partial}{\partial t} (\nabla \times \underline{u}) + \nabla \times (\underline{u} \times \nabla \times \underline{u}) = 0$$

AT $t = t_0$, WE HAVE:

$$\frac{\partial}{\partial t} (\nabla \times \underline{u}) = 0$$

$\Rightarrow \nabla \times \underline{u}$ MUST REMAIN CONSTANT, I.E.O.